examples/RedBlack/attic.v
@@ -1,0 +1,96 @@
+Definition showDiscards (r : Result) :=
+  match r with
+  | Success ns nd _ _ => "Success: number of successes " ++ show ns ++ newline ++
+                         "         number of discards "  ++ show nd ++ newline
+  | _ => showResult r
+  end.
+
+Definition testInsertNaiveShowDiscards :=
+  showDiscards (quickCheck (insert_is_redblack_checker genAnyTree)).
+
+(* QuickCheck testInsertNaiveShowDiscards. *)
+
+(* CH: the following implementation seems to me rather inefficient
+   (quadratic in the tree height); there seems to be too much
+   redundancy between the two fixpoints (as shown formally by
+   has_black_height), can't they be merged? Or can't at least the
+   checks in black_height be all removed?
+
+   Matt Might has a simpler and more efficient implementation:
+   http://matt.might.net/articles/quick-quickcheck/
+   Implemented above as is_redblack_bool
+   That is simpler and much more efficient (overall time: 5.19s vs 8.53s) *)
+
+Fixpoint is_redblack_bool (t : tree) (c: color) : bool  :=
+  match t with
+    | Leaf => true
+    | Node c' tl _ tr =>
+      match c' with
+        | Black =>
+          (black_height_bool tl == black_height_bool tr) &&
+          is_redblack_bool tl Black && is_redblack_bool tr Black
+        | Red =>
+          match c with
+            | Black =>
+              (black_height_bool tl == black_height_bool tr) &&
+              is_redblack_bool tl Red && is_redblack_bool tr Red
+            | Red => false
+          end
+      end
+  end.
+
+Lemma has_black_height :
+  forall t c, is_redblack_bool t c -> exists n, black_height_bool t = Some n.
+Proof.
+  move=> t. induction t; move => c' Hdec; first by exists 0.
+  destruct c'; destruct c; simpl in *; (try by discriminate);
+  move/andP: Hdec => [/andP [/eqP Heq  /IHt1 [n1 Ht1]]  /IHt2 [n2 Ht2]];
+  remember (black_height_bool t1) as h1;
+  remember (black_height_bool t2) as h2;
+  destruct h1, h2; (try discriminate);
+  inversion Heq; subst; eexists; by rewrite eq_refl.
+Qed.
+
+Lemma is_redblackP :
+  forall (t : tree) (c : color) n,
+    reflect (is_redblack t c n)
+            (is_redblack_bool t c && (black_height_bool t == Some n)).
+Proof.
+  move => t c n.
+  apply (@iffP (is_redblack_bool t c && (black_height_bool t == Some n)));
+    first by apply/idP.
+  - move: c n. induction t; intros c' n' Hrb.
+    + move/andP : Hrb => [_ /= /eqP [Hn]]; subst. by constructor.
+    + move/andP : Hrb => [Hdec /eqP Hheight].
+      destruct c'; destruct c; simpl in *; (try by discriminate);
+      move/andP: Hdec => [/andP [/eqP Heq  Ht1]  Ht2];
+      remember (black_height_bool t1) as h1;
+      remember (black_height_bool t2) as h2;
+      destruct h1, h2; (try discriminate);
+      inversion Heq; subst; rewrite eq_refl in Hheight;
+      inversion Hheight; subst;
+      constructor;
+      (try by (apply IHt1; apply/andP; split => //));
+      by (apply IHt2; apply/andP; split => //).
+  - move=> Hrb. induction Hrb; (try by reflexivity);
+    move/andP: IHHrb1 => [Htl /eqP Hhtl];
+    move/andP: IHHrb2 => [Htr /eqP Hhtr]; subst; simpl;
+    rewrite Hhtl Hhtr; repeat (apply/andP; split => //);
+    by rewrite eq_refl.
+Qed.
+
+Lemma is_redblack_exP :
+  forall (t : tree) (c : color),
+    reflect (exists n, is_redblack t c n)
+            (is_redblack_bool t c).
+Proof.
+  move=> t c.
+  apply (@iffP (is_redblack_bool t c));
+    first by apply/idP.
+  - move=> Hrb.  move/has_black_height: (Hrb) => [n Hh]. exists n.
+    apply/is_redblackP. apply/andP; split. exact Hrb.
+      by apply/eqP.
+  - by move => [n /is_redblackP/andP [Hrb _]].
+Qed.
+
+*)
