examples/RedBlack/verif.v
@@ -1,0 +1,120 @@
+Require Import ssreflect ssrnat ssrbool eqtype.
+
+Require Import List String.
+
+Require Import QuickChick.
+Require Import SetOfOutcomes EndToEnd.
+
+Require Import redblack.
+Require Import testing.
+
+Lemma is_redblackP :
+  forall (t : tree),
+    reflect (is_redblack t)
+            (is_redblack_bool t).
+Proof.
+  move => t. induction t.
+  - constructor. rewrite /is_redblack. exists 0. by constructor.
+  - admit.
+Admitted. (* TODO *)
+
+Lemma genColor_correct:
+  genColor <--> (fun _ => True).
+Proof.
+  rewrite /genColor. intros c. rewrite elements_equiv.
+  split => // _. left.
+  destruct c;  by [ constructor | constructor(constructor)].
+Qed.
+
+(* ugly proof, needs refactoring at some point *)
+Lemma genRBTree_height_correct:
+  forall c h,
+    (genRBTree_height h c) <--> (fun t => is_redblack' t c h).
+Proof.
+  move => c h. move : c. induction h as [| h]; intros c' t.
+  { rewrite /genRBTree_height. split.
+    - destruct c'.
+      + rewrite returnGen_def. by move => <-; constructor.
+      + rewrite oneof_equiv. move => [[gen [H Hgen]] | [// H Hret]].
+        inversion H as [HIn | HIn]; subst.
+        * rewrite returnGen_def in Hgen; subst. by constructor.
+        * inversion HIn as [HIn' |  HIn'] => //; subst.
+        move: Hgen => [n [Hn Hret]]. rewrite returnGen_def in Hret; subst.
+          by constructor; constructor.
+    - move=> H. inversion H; subst.
+      + destruct c' => //. rewrite oneof_equiv. left.
+        eexists. by split; [by apply in_eq |].
+      + rewrite oneof_equiv. left. eexists.
+        split. by constructor(apply in_eq).
+        eexists. split; first by apply arbNat_correct.
+        inversion H0; subst. inversion H1; subst.
+        reflexivity. }
+  { split.
+    - destruct c'.
+      + move => [tl [/IHh Hgentl [tr [/IHh Hgentr [n [_ H]]]]]].
+        rewrite returnGen_def in H; subst.
+        by constructor => //.
+      + move => [[] [Hcol Hgen]].
+        * move : Hgen =>
+          [tl1 [/IHh Htl1 [tl2 [/IHh Htl2 [tr1 [/IHh Htr1 [tr2 [/IHh Htr2 H]]]]]]]].
+          move : H => [n [_ [nl [_ [nr [_ H]]]]]].
+          rewrite returnGen_def in H; subst.
+          constructor; constructor=> //.
+       * move : Hgen => [tl [/IHh Hgentl [tr [/IHh Hgentr [n [_ H]]]]]].
+         rewrite returnGen_def in H; subst.
+         constructor => //.
+    - move => H. inversion H as [| n tl tr h' Hrbl Hrbr |
+                                   c n tl tr h' Hrbl Hrbr]; subst.
+      + inversion Hrbl as [| |c n1 tl1 tr1 h1 Hrbl1 Hrbr1]; subst.
+        inversion Hrbr as [| |c n2 tl2 tr2 h2 Hrbl2 Hrbr2]; subst.
+        exists Red. split; first by apply genColor_correct.
+        exists tl1. split; first by apply IHh.
+        exists tl2. split; first by apply IHh.
+        exists tr1. split; first by apply IHh.
+        exists tr2. split; first by apply IHh.
+        exists n. split; first by apply arbNat_correct.
+        exists n1. split; first by apply arbNat_correct.
+        exists n2. split; first by apply arbNat_correct.
+        reflexivity.
+      + destruct c'.
+        * exists tl. split; first by apply IHh.
+          exists tr. split; first by apply IHh.
+          exists n. split; first by apply arbNat_correct.
+          reflexivity.
+        * exists Black. split; first by apply genColor_correct.
+          exists tl. split; first by apply IHh.
+          exists tr. split; first by apply IHh.
+          exists n. split; first by apply arbNat_correct.
+          reflexivity. }
+Qed.
+
+Lemma genRBTree_correct:
+  genRBTree <--> is_redblack.
+Proof.
+  move => t. split.
+  - rewrite /genRBTree sized_def.
+    move => [n /genRBTree_height_correct Hgen].
+    eexists. eassumption.
+  - rewrite /is_redblack. move => [h /genRBTree_height_correct  Hgen].
+    rewrite /genRBTree sized_def. by exists h.
+Qed.
+
+Lemma insert_is_redblack_checker_correct:
+  semChecker (insert_is_redblack_checker genRBTree) <-> insert_preserves_redblack.
+Proof.
+  rewrite /insert_is_redblack_checker /insert_preserves_redblack semForAll.
+  split.
+  + move => H x s Hrb.
+    have /H/semPredQProp/semForAll H' : @arbitraryNat Pred _ x
+      by apply arbNat_correct.
+    have /H'/semPredQProp/semImplication H'': @genRBTree Pred _ s
+      by apply genRBTree_correct.
+    apply/is_redblackP.
+    by move/is_redblackP/H''/semBool: Hrb.
+  + move=> H a _.
+    apply/semPredQProp/semForAll. move => t Hgen.
+    apply/semPredQProp/semImplication. move => Hrb.
+    apply/semBool. apply/is_redblackP.
+    move: Hrb => /is_redblackP [n Hrb]. eapply H.
+    eexists. eassumption.
+Qed.
